formal_verification/QEDFV/Typing/Elaboration.lean
@@ -1,4 +1,5 @@
 import QEDFV.Signature.ScopedStack
+import QEDFV.Signature.ConstSchemes
 
 namespace QEDFV
 
@@ -18,5 +19,32 @@ inductive Elaborates : ScopeStack -> Term -> RTerm -> Prop where
       (hx : Elaborates s x rx) : Elaborates s (.comb f x) (.rComb rf rx)
   | abs {s n ty b rb}
       (hb : Elaborates s b rb) : Elaborates s (.abs n ty b) (.rAbs n ty rb)
+
+inductive ElaboratesWithInstances (env : ConstSchemeEnv) : ScopeStack -> Term -> RTerm -> Prop where
+  | var (s n ty) :
+      ElaboratesWithInstances env s (.var n ty) (.rVar n ty)
+  | const {s n ty}
+      (hlookup : lookup s n = some ty)
+      (hInst : admissibleConstInstance env n ty) :
+      ElaboratesWithInstances env s (.const n ty) (.rConst n ty)
+  | comb {s f x rf rx}
+      (hf : ElaboratesWithInstances env s f rf)
+      (hx : ElaboratesWithInstances env s x rx) :
+      ElaboratesWithInstances env s (.comb f x) (.rComb rf rx)
+  | abs {s n ty b rb}
+      (hb : ElaboratesWithInstances env s b rb) :
+      ElaboratesWithInstances env s (.abs n ty b) (.rAbs n ty rb)
+
+theorem elaborates_const_instance
+    (env : ConstSchemeEnv)
+    (s : ScopeStack)
+    (n : ConstName)
+    (ty tyGen : HolType)
+    (hLookupScope : lookup s n = some ty)
+    (hLookupScheme : lookupConstScheme env n = some tyGen)
+    (hInst : TyInstance ty tyGen) :
+    ElaboratesWithInstances env s (.const n ty) (.rConst n ty) := by
+  exact ElaboratesWithInstances.const hLookupScope
+    (const_instance_from_principal env n tyGen ty hLookupScheme hInst)
 
 end QEDFV
